Explained subroutines more

SubroutineSimple.v
@@ -9,34 +9,68 @@ Require Import ObsTrace.
 
 (* A Domain is an annotation on a component or set of components reflecting its
    relationship to the program state. Domains are nested, so a domain can be subsumed by
-   a higher domain, and all of its components with it. For instance, a stack in a coroutine
-   system has a domain containing all of the addresses in the stack's range, and the frames
-   pushed on the stack each have their own, as described below. *)
-Section DOMAIN_MODEL.
+   a higher domain, and all of its components with it.
 
+   First, an example of stack domains. Suppose we have a stack resulting from caller A
+   calling callee B. The stack looks like this:
+               sp
+   -----------------------------------------------
+   | A's frame | Empty stack..................
+   -----------------------------------------------
+        a1                      a2
+
+   B's frame is not yet allocated until it sets the stack pointer, but B
+   has access to everything above the current stack pointer. So lets consider the status of
+   addresses a1 and a2 in the moment B gains control.
+
+   a1 is in a frame that is currently inaccessible, but someday - after B returns - will
+   again be active. a2 is still in the accessible part of the stack. If B makes another call,
+   say to a functin C, we will have:
+
+                            sp
+   -----------------------------------------------
+   | A's frame | B's frame  | Empty.....
+   -----------------------------------------------
+        a1        a2
+
+   a1 and a2 are both inaccessible. But a2 will be accessible again on the next return.
+   Whereas a1 will be inaccesible still, until the return after (assuming no further calls.)
+   So in a stack domain, an Inaccessible domain carries a nested stack domain that is the one
+   that will be used after the next unmatched return.
+ *)
+
+Section DOMAIN_MODEL.
+  (* Outside is non-stack memory and registers. Inaccessible and Accessible are as described above. *)
   Inductive StackDomain :=
-  | Inactive (sd:StackDomain)
-  | Active
+  | Inaccessible (sd:StackDomain)
+  | Accessible
   | Outside
   .
 
-  (* Finally we need a way to map components to the domain they belong to. *)
+  (* All components belong to domain, and a domain map tells us which. *)
   Definition DomainMap := Component -> StackDomain.
   
 End DOMAIN_MODEL.
 
 Section WITH_MAPS.
 
-  Variable cdm : CodeMap'.
-  Variable sm : Addr -> bool.
-  Variable pOf : MachineState -> PolicyState.
-  
-  Definition initD : DomainMap * nat :=
+  Variable cdm : CodeMap'. (* Map of where code lives in memory and its annotation. *)
+  Variable sm : Addr -> bool. (* Determines whether an address is in the stack. *)
+  Variable pOf : MachineState -> PolicyState. (* Policy initialization function. *)
+
+  (* We will use the machinery defined at the end of Machine.v to extend traces of the
+     machine with context that will inform our properties. In this case the context is a
+     pair of a Domain Map and a natural number representing the depth of the stack. *)
+  Definition context : Type := DomainMap * nat.
+
+  (* For the initial context, we construct a domain map that maps the stack to Accessible
+     and everything else to Outside. The stack depth is 0. *)
+  Definition initC : context :=
     let dm := fun k =>
                 match k with
                 | Mem a =>
                   if sm a
-                  then Active
+                  then Accessible
                   else Outside
                 | _ => Outside
                 end in
@@ -44,28 +78,11 @@ Section WITH_MAPS.
   
   (* Our update function checks an "annotation" on the code being executed.
      Annotations are defined in Machine.v as an alternative to a million different
-     maps, and the ones that matter are call, return, yield, and share.
+     maps, and the ones that matter here are call and return.
 
      Annotations are given by the compiler. We assume that the compiler can tell us
-     which instructions represent calls, returns, and yields. Shares are more complicated;
-     the compiler cannot directly tell us which component(s) are being shared, because sharing
-     is often dynamic. What it can do is identify a relation between the machine state
-     and the component(s) being shared.
-     
-     For an example, suppose that a caller is sharing an address as an argument to its callee.
-     It executes a store instruction that the compiler identifies as a share; the target of
-     the share is the address to which the argument is being stored, held within the appropriate
-     register. So, we would relate a given machine state to the contents of the register in that
-     state.
-     
-     This is a much stronger assumption of information from the compiler than we had before!
-     We now fully rely on the compiler to recognize returns, for instance. Relating returns
-     to the actual program state is the job of control flow property, WBCF.
-
-     Note that yields don't actually change the domain map, as they don't change which
-     addresses belong to which stacks. *)
-  
-  Definition updateD (m:MachineState) (prev:DomainMap*nat) : DomainMap * nat :=
+     which instructions represent calls and returns. *)
+  Definition updateC (m:MachineState) (prev:context) : context :=
     let '(dm, d) := prev in
     match AnnotationOf cdm (m (Reg PC)) with
     | Some call => (* A call adjusts the domain map by marking the caller's frame "inactive" *)
@@ -75,7 +92,7 @@ Section WITH_MAPS.
                     | _, Outside => Outside
                     | Mem a, sd =>
                       if wlt a (m (Reg SP))
-                      then Inactive sd
+                      then Inaccessible sd
                       else sd
                     | _, _ => Outside
                     end in
@@ -83,21 +100,27 @@ Section WITH_MAPS.
     | Some ret => (* A return unwraps the outermost domain of all components in the initial stack *)
       let dm' := fun k =>
                     match dm k with
-                    | Inactive sd => sd
+                    | Inaccessible sd => sd
                     | _ => dm k
                     end in
       (dm', d-1)
     | _ => (dm, d)
     end.
 
+  (* Now it's quite simple to define an "ultra eager" integrity property:
+     if we run from any initial state, updating the context as above, then
+     at any particular state where a component k is in an Inaccessible domain,
+     k has the same value in the following state (if any.) We term this property
+     ultra eager because it "checks" at each step that components that are inaccessible
+     don't change, the most frequent it is possible to check. *)
   Definition SimpleStackIntegrityUE : Prop :=
     forall minit MCP k sd mcp mcp',
-      WithContextMP updateD initD (MPTraceOf (minit, pOf minit)) MCP ->
+      WithContextMP updateC initC (MPTraceOf (minit, pOf minit)) MCP ->
       ContextSegment (fun _ _ => False) MCP (notfinished mcp (finished mcp')) ->
-      fst (cstate mcp) k = Inactive sd ->
+      fst (cstate mcp) k = Inaccessible sd ->
       mstate mcp k = mstate mcp' k.
 
-    (* We can do a similar Ultra Eager style property with confidentiality, and since we're
+    (* We can do a similar ultra eager style property with confidentiality, and since we're
        not allowing sharing it is straightforward. But some preliminaries on confidentiality.
        Firstly: confidentiality is expressed in terms of "variant" states. A K-variant
        state of m is a state that agrees with m at every component not in the set K. It may also
@@ -113,44 +136,118 @@ Section WITH_MAPS.
     forall k,
       (m k <> m' k \/ n k <> n' k) ->
       m' k = n' k.
-  
-  Definition SimpleStackConfidentialityUE : Prop :=
-    forall minit MCP sd mcp mcp' n n' o,
-      WithContextMP updateD initD (MPTraceOf (minit, pOf minit)) MCP ->
-      ContextSegment (fun _ _ => False) MCP (notfinished mcp (finished mcp')) ->
-      variantOf (fun k => fst (cstate mcp) k = Inactive sd) (mstate mcp) n ->
-      step (mstate mcp) = (mstate mcp', o) ->
-      step n = (n',o) /\ sameDifference (mstate mcp) (mstate mcp') n n'.
 
+  (* Once again, we take adjacent pairs of states in the trace from an arbitrary
+     start state and check that a property holds between them. In this case, that
+     in any K-variant of the first state where K is the set of components that are
+     Inacessible in that state, the step has the same observable behavior and makes
+     the same changes to state. *)
+  Definition SimpleStackConfidentialityUE : Prop :=
+    forall minit MCP sd m dm d p m' dm' d' p' n o n' p'' o',
+      WithContextMP updateC initC (MPTraceOf (minit, pOf minit)) MCP ->
+      ContextSegment (fun _ _ => False) MCP (notfinished (m,(dm,d),p) (finished (m',(dm',d'),p'))) ->
+      variantOf (fun k => dm k = Inaccessible sd) m n ->
+      mpstep (m,p) = Some (m',p',o) ->
+      mpstep (n,p) = Some (n',p'',o') ->
+      sameDifference m m' n n' /\ p = p'' /\ o = o'.
+
+  (* Here are some helper relations to combine the addition of context to a trace,
+     and the segmenting of the resulting trace by a proposition P.*)
   Definition FindSegmentMP P mp dm MCP :=
     exists MCP',
-      WithContextMP updateD dm (MPTraceOf mp) MCP' /\
+      WithContextMP updateC dm (MPTraceOf mp) MCP' /\
       ContextSegment P MCP' MCP.
 
   Definition FindSegmentM P m dm MC :=
     exists MC',
-      WithContextM updateD dm (MTraceOf m) MC' /\
+      WithContextM updateC dm (MTraceOf m) MC' /\
       ContextSegmentM P MC' MC.
+
+  (* For integrity, ultra eager properties are significantly stronger than we actually
+     need. In fact, we want to consider lazy policies that allow illegal writes at times
+     in the name of efficiency. So we should consider what our actual goal is here - what
+     use are these properties? Here is an example of how we might think of a program logic
+     call rule that lets us guarantee that from a call point, if execution returns to the
+     caller, Inaccessible components are preserved. *)
+  Inductive StepsTo : MachineState -> MachineState -> Prop :=
+  | isNow : forall m, StepsTo m m
+  | stepsTo : forall m1 m2 m' o,
+      step m1 = (m',o) ->
+      StepsTo m' m2 ->
+      StepsTo m1 m2.
+  
+  Definition CallRule : Prop :=
+    forall minit MCP mcall dmcall dcall pcall,
+      WithContextMP updateC initC (MPTraceOf (minit, pOf minit)) MCP ->
+      InTrace (mcall,(dmcall,dcall),pcall) MCP ->
+      AnnotationOf cdm (mcall (Reg PC)) = Some call ->
+         (* Case 1: Divergence (including due to failstop) *)
+      (forall MCP' m' dm d p',
+          WithContextMP updateC (dmcall,dcall) (MPTraceOf (mcall,pcall)) MCP' ->
+          InTrace (m',(dm,d),p') MCP' ->
+          d > dcall)
+      \/ (* Case 2: Return *)
+      (exists m',
+          StepsTo mcall m' /\
+          forall k sd,
+            dmcall k = Inaccessible sd ->
+            mcall k = m' k).
+
+  (* We could use this as our ultimate specification, or just to guide our trace
+     properties. Note that this rule cares nothing for what happens to the state of
+     the Inaccessible components during the call, only that whe we return, they are
+     the same. Our eager property reflects this; instead of guaranteeing that they never
+     change, it guarantees that they are unchanged if and when the function returns. *)
   
   Definition SimpleStackIntegrityEager : Prop :=
     forall minit MCP d k sd mcp mcp',
-      FindSegmentMP  (fun m c => snd c = d) (minit, pOf minit) initD MCP ->
+      FindSegmentMP  (fun m c => snd c = d) (minit, pOf minit) initC MCP ->
       mcp = head MCP ->
-      fst (cstate mcp) k = Inactive sd ->
+      fst (cstate mcp) k = Inaccessible sd ->
       Last MCP mcp' ->
       mstate mcp k = mstate mcp' k.
-  
-  Definition Stuck (MCP : @MCPTrace (DomainMap*nat)) : Prop :=
-    exists m c p,
-      Last MCP (m,c,p) ->
-      mpstep (m,p) = None.
 
+  Theorem EagerIntSufficient :
+    SimpleStackIntegrityEager ->
+    CallRule.
+  Proof.
+  Admitted.
+  
+  (* We can make a similar argument about confidentiality, though it may be odd to
+     think of a confidentiality call rule. We can at least think of the following as
+     the "caller's view" of confidentiality: that from the call to the return, its
+     Inaccessible memory ought change nothing about the observable behavior of the
+     machine, and if control returns, its Inaccessible memory also did not impact the
+     returned state. *)
+
+  Definition ConfRule : Prop :=
+    forall minit MCP mcall dmcall dcall pcall n MCP' N MO NO,
+      WithContextMP updateC initC (MPTraceOf (minit, pOf minit)) MCP ->
+      InTrace (mcall,(dmcall,dcall),pcall) MCP ->
+      AnnotationOf cdm (mcall (Reg PC)) = Some call ->
+      variantOf (fun k => exists sd, dmcall k = Inaccessible sd) mcall n ->
+      (* Clause 1: output up to return identical *)
+      PrefixUpTo (fun '(_,(dm,d),_) => d = dcall) MCP MCP' ->
+      FindSegmentM (fun _ '(dm,d) => d = dcall) n (dmcall,dcall) N ->
+      ObsOfMCP MCP' MO ->
+      ObsOfMC N NO ->
+      ObsOfMP MO ~=_O ObsOfM NO /\
+      (* Clause 2: if return, then state changes the same *)
+      (forall m' dm' p',
+          Last MCP' (m',(dm',dcall),p') ->
+          exists n' dm'',
+            Last N (n',(dm'',dcall)) /\
+            sameDifference mcall m' n n').
+
+  (* The flip side of the caller's rule is the trace property that holds on subtraces
+     representing calls. This only needs to be strong enough to support the caller-side
+     reasoning, so here is an example of such an eager (but not ultra-eager) property. *)
   Definition SimpleStackConfidentialityEager : Prop :=
     forall minit M MO d sd m dm p n N NO,
       let P := (fun m c => snd c = d) in
-      FindSegmentMP P (minit, pOf minit) initD M ->
+      FindSegmentMP P (minit, pOf minit) initC M ->
       head M = (m,(dm,d),p) ->
-      variantOf (fun k => dm k = Inactive sd) m n ->
+      variantOf (fun k => dm k = Inaccessible sd) m n ->
       FindSegmentM P n (dm,d) N ->
       ObsOfMCP M MO ->
       ObsOfMC N NO ->
@@ -166,40 +263,73 @@ Section WITH_MAPS.
       (Infinite M ->
        ObsOfMP MO ~=_O ObsOfM NO)
       /\ (* Case 3 *)
-      (Stuck M ->
-       ObsOfMP MO <=_O ObsOfM NO).
+      (forall mend dmend pend,
+          Last M (mend, dmend, pend) ->
+          P mend (dm,d) ->
+          ObsOfMP MO <=_O ObsOfM NO).
 
-  Inductive StepsTo : MachineState -> MachineState -> Prop :=
-  | isNow : forall m, StepsTo m m
-  | stepsTo : forall m1 m2 m' o,
-      step m1 = (m',o) ->
-      StepsTo m' m2 ->
-      StepsTo m1 m2.
-
-  Definition CallRule : Prop :=
-    forall minit MCP mcall dmcall dcall pcall,
-      WithContextMP updateD initD (MPTraceOf (minit, pOf minit)) MCP ->
-      InTrace (mcall,(dmcall,dcall),pcall) MCP ->
-      AnnotationOf cdm (mcall (Reg PC)) = Some call ->
-         (* Case 1: Divergence (including due to failstop) *)
-      (forall MCP' m' dm d p',
-          WithContextMP updateD (dmcall,dcall) (MPTraceOf (mcall,pcall)) MCP' ->
-          InTrace (m',(dm,d),p') MCP' ->
-          d > dcall)
-      \/ (* Case 2: Return *)
-      (exists m',
-          StepsTo mcall m' /\
-          (forall k sd,
-            dmcall k = Inactive sd ->
-            mcall k = m' k) /\
-          (forall n k,
-              variantOf (fun k' => exists sd, dmcall k = Inactive sd) mcall n ->
-              StepsTo n m')).
-
-  Theorem EagerSufficient :
-    SimpleStackIntegrityEager ->
+  Theorem EagerConfSufficient :
     SimpleStackConfidentialityEager ->
-    CallRule.
+    ConfRule.
+  Proof.
+  Admitted.
+
+  (* Now the above properties do a few things all at once that it helps to disentangle. They
+     quantify over all initial states, then over all segments of a trace at or above a certain
+     depth on the stack, ending with the return when the depth is reduced. And they state
+     properties of those segments. Lets focus on just capturing what it means for a trace
+     to respect the integrity and confidentiality of components, and separate out the finding
+     of the traces. The predicate K will indicate the set of components that must be protected. *)
+
+  Definition TraceIntegrityEager (K : Component -> Prop) (MCP:MCPTrace) : Prop :=
+    forall k (mcp':@MCPState context),
+      K k->
+      Last MCP mcp' ->
+      mstate (head MCP) k = mstate mcp' k.
+
+  (* The confidentiality trace property needs to know when the variant trace can be considered to have
+     returned, for which it takes a predicate on states and contexts, P. *)
+  Definition TraceConfidentialityEager (K : Component -> Prop)
+             (P:MachineState -> context -> Prop)
+             (MCP:@MCPTrace context) : Prop :=
+    forall MCP MO d m dm p n N NO,
+      head MCP = (m,(dm,d),p) ->
+      variantOf K m n ->
+      FindSegmentM P n (dm,d) N ->
+      ObsOfMCP MCP MO ->
+      ObsOfMC N NO ->
+         (* Case 1 *)
+      (forall mend dmend pend,
+          Last MCP (mend,dmend,pend) ->
+          ~ P mend (dm,d) ->
+          exists nend dnend,
+            Last N (nend,dnend) /\
+            ObsOfMP MO ~=_O ObsOfM NO /\
+            sameDifference m mend n nend)
+      /\ (* Case 2 *)
+      (Infinite MCP ->
+       ObsOfMP MO ~=_O ObsOfM NO)
+      /\ (* Case 3 *)
+      (forall mend dmend pend,
+          Last MCP (mend, dmend, pend) ->
+          P mend (dm,d) ->
+          ObsOfMP MO <=_O ObsOfM NO).
+
+  (* Now we can quantify over all initial states and segments starting with calls,
+     to create a property of the system that all calls enjoy both confidentiality and
+     integrity. *)
+  Definition StackSafety :=
+    forall minit MCP m dm d p,
+      let P := (fun m '(dm, d') => d' >= d) in
+      FindSegmentMP P (minit, pOf minit) initC MCP ->
+      head MCP = (m,(dm,d),p) ->
+      let K := (fun k => exists sd, dm k = Inaccessible sd) in
+      TraceIntegrityEager K MCP /\
+      TraceConfidentialityEager K P MCP.
+
+  Theorem StackSafetySufficient :
+    StackSafety ->
+    CallRule /\ ConfRule.
   Proof.
   Admitted.
 
